---
title:  "Normal Distribution"
excerpt: "가우시안 정규분포의 성질들"
categories:
  - Mathematical_Testing
last_modified_at: 2021-11-11

toc: true
toc_label: "Table Of Contents"
toc_icon: "cog"
toc_sticky: true

use_math: true
---

 기초가 되는 Normal 분포의 성질을 연구해봅시다.
{: .notice--warning}

# [Normal Distribution](#link){: .btn .btn--primary}{: .align-center}

> ## Definition 5 : Normal DIstribution

> Definition

A normal distribution with mean $\mu$ and variance $\sigma^{2}$ is a continuous distribution with probability density function

$$f(x)=\frac{1}{\sigma \sqrt{2 \pi}} e^{-\frac{1}{2 \sigma^{2}}(x-\mu)^{2}}$$

> ## Theorem 10 : Normal and constant

> Definition

If $X \sim N\left(\mu, \sigma^{2}\right)$, and a and $b$ are finite constants, then

$$Y=a X+b \sim N\left(a \mu+b, a^{2} \sigma^{2}\right)$$

> **proof (a>0)**

- $a>0$ 에 대하여 Cumulative density function of Y 는

$$\begin{aligned}
F_{Y}(y) &=P(Y \leq y) \\
&=P(a X+b \leq y) \\
&=P\left(X \leq \frac{y-b}{a}\right) \\
&=F_{X}\left(\frac{y-b}{a}\right)
\end{aligned}$$

- 이떄 CDF 를 미분하면 pdf 를 얻을 수 있으므로 다음과 같은 식을 얻습니다.

$$\begin{aligned}
f_{Y}(y) &=\frac{d}{d y} F_{X}\left(\frac{y-b}{a}\right) \\
&=\frac{1}{a} f_{X}\left(\frac{y-b}{a}\right)
\end{aligned}$$

- 이떄 $X \sim N(\mu , \sigma^2)$ 이므로

$$\begin{aligned}
f_{Y}(y) &=\frac{1}{a}\left[\frac{1}{\sigma \sqrt{2 \pi}} e^{-\frac{1}{2 \sigma^{2}}\left(\left(\frac{y-b}{a}\right)-\mu\right)^{2}}\right] \\
&=\frac{1}{(a \sigma) \sqrt{2 \pi}} e^{-\frac{1}{2(a \sigma)^{2}}(y-[b+a \mu])^{2}}
\end{aligned}$$

- 이때 위 분포는 평균 $a\mu +b $ 와 분산 $a^2 \sigma^2$ 를 가지는 Normal 분포입니다. 

> **proof (a<0)**

$$\begin{aligned}
F_{Y}(y) &=P(Y \leq y) \\
&=P(a X+b \leq y) \\
&=P\left(X \geq \frac{y-b}{a}\right) \\
&=1-F_{X}\left(\frac{y-b}{a}\right)
\end{aligned}$$

- cdf 를 미분하면 pdf 이므로 

$$\begin{aligned}
f_{Y}(y) &=\frac{d}{d y}\left[1-F_{X}\left(\frac{y-b}{a}\right)\right] \\
&=\frac{1}{a} f_{X}\left(\frac{y-b}{a}\right)
\end{aligned}$$

$$\begin{aligned}
f_{Y}(y) &=\frac{1}{a}\left[\frac{1}{\sigma \sqrt{2 \pi}} e^{\left.-\frac{1}{2 \sigma^{2}}\left(\left(\frac{y-b}{a}\right)-\mu\right)^{2}\right]}\right] \\
&=\frac{1}{(a \sigma) \sqrt{2 \pi}} e^{-\frac{1}{2(a \sigma)^{2}}(y-[b+a \mu])^{2}}
\end{aligned}$$

- 위 값 역시 평균 $a\mu +b $ 와 분산 $a^2 \sigma^2$ 를 가지는 Normal 분포입니다. 

> ## Corollary 3 : Standard Normal Expression

> Corollary

$$\text { If } X \sim N\left(\mu, \sigma^{2}\right), X \text { can be expressed as } X=\sigma Z+\mu \text { where } Z \sim N(0,1)$$

> **proof**

If $Z \sim N(0,1)$, then $X=\sigma Z+\mu$ would be distributed $N\left(0 \cdot \sigma+\mu, \sigma^{2} \cdot 1\right)$ or $N\left(\mu, \sigma^{2}\right)$ by Theorem 10 .

> ## Theorem 11 : Standard Normal and mgf

> Theorem

A standard normal distribution, see Definition 6, has mgf
$$
M(t)=e^{t^{2} / 2}
$$

> Proof

- Definition 5 , 6 에 의하여 Standard Normal DIstribution 의 pdf 는 다음과 같습니다.

$$f(x)=\frac{1}{\sqrt{2 \pi}} e^{-x^{2} / 2}$$

- 이제 MGF 를 직접 계산해봅시다.

$$\begin{aligned}
M(t) &=\int_{-\infty}^{\infty} e^{t x} \cdot \frac{1}{\sqrt{2 \pi}} e^{-x^{2} / 2} d x \\
&=\int_{-\infty}^{\infty} \frac{1}{\sqrt{2 \pi}} e^{t x-x^{2} / 2} d x \\
&=\int_{-\infty}^{\infty} \frac{1}{\sqrt{2 \pi}} e^{-\frac{1}{2}\left(x^{2}-2 t x+(-t)^{2}\right)+\frac{t^{2}}{2}} d x \\
&=e^{\frac{t^{2}}{2} \int^{\infty} \frac{1}{\sqrt{2 \pi}} e^{-\frac{1}{2}}\left(x-\frac{t}{4}\right)^{2} d x} \\
&=e^{t^{2} / 2} \cdot 1
\end{aligned}$$

- 위에서 $$\frac{1}{\sqrt{2 \pi}} e^{-\frac{1}{2}\left(x-\frac{t}{4}\right)^{2}}$$ 는 N(t/4 , 1) 의 pdf 이므로 integral 은 1이 됩니다.

> ## Corrolary 4 : MFG of Normal

> Corollarray

If $X \sim N\left(\mu, \sigma^{2}\right)$, then the moment generating function is

$$M(t)=e^{\mu t} e^{\sigma^{2} t^{2} / 2}$$

> Proof

Proof. If $X \sim N\left(\mu, \sigma^{2}\right)$, then $X=\sigma Z+\mu$ where $Z \sim N(0,1)$ by Corollary 3 . Then Theorem 8 can be used.

$$\begin{aligned}
M_{X}(t) &=M_{\sigma Z+\mu}(t) \\
&=e^{\mu t} M_{Z}(\sigma t) \\
&=e^{\mu t} e^{(\sigma t)^{2} / 2} \\
&=e^{\mu t} e^{\sigma^{2} t^{2} / 2}
\end{aligned}$$

> ## Theorem 12 : X+Y distribution

> theorem

If $X \sim N\left(\mu, \sigma^{2}\right)$ and $Y \sim N\left(\nu, \tau^{2}\right)$ and $X$ and $Y$ are independent, then

$$X+Y \sim N\left(\mu+\nu, \sigma^{2}+\tau^{2}\right)$$

> Proof

By Theorem 9 ,

$$\begin{aligned}
M_{X+Y}(t) &=M_{X}(t) M_{Y}(t) \\
&=\left[e^{\mu t} e^{\sigma^{2} t^{2} / 2}\right]\left[e^{\nu t} e^{\tau^{2} t^{2} / 2}\right] \\
&=e^{\mu t+\nu t} e^{\sigma^{2} t^{2} / 2+\tau^{2} t^{2} / 2} \\
&=e^{(\mu+\nu) t} e^{\left(\sigma^{2}+\tau^{2}\right) t^{2} / 2}
\end{aligned}$$

We see that $M_{X+Y}(t)$ is the moment generating function of a normal distribution with mean $\mu+\nu$ and variance $\sigma^{2}+\tau^{2}$. Therefore by the uniqueness of moment generating functions, Proposition 1 ,

$$X+Y \sim N\left(\mu+\nu, \sigma^{2}+\tau^{2}\right)$$

> ## Theorem 13 : Standard Transformation

> defitition 

If $X$ is a normally distributed random variable with mean $\mu$ and standard deviation $\sigma$, then $Z=\frac{X-\mu}{\sigma}$ has a standard normal distribution.

> Proof

PROOF. By Corollary 4 ,

$$M_{X}(t)=e^{\mu t} e^{\sigma^{2} t^{2} / 2}$$

Then

$$\begin{aligned}
M_{Y}(t) &=M_{X-\mu}(t) \\
&=M_{(1 / \sigma) X-(\mu / \sigma)}(t) \\
&=e^{(-\mu / \sigma) t} M_{X}\left(\frac{1}{\sigma} t\right)
\end{aligned}$$

by Theorem 8 . Then

$$\begin{aligned}
M_{Y}(t) &=e^{(-\mu / \sigma) t}\left[e^{\mu\left(\frac{1}{\sigma} t\right)} e^{\sigma^{2}\left(\frac{1}{\sigma} t\right)^{2} / 2}\right] \\
&=e^{(-\mu / \sigma) t}\left[e^{(\mu / \sigma) t} e^{\sigma^{2} \cdot \frac{1}{\sigma^{2}} \cdot t^{2} / 2}\right] \\
&=e^{(-\mu / \sigma+\mu / \sigma) t} e^{1 \cdot t^{2} / 2} \\
&=e^{0 t} e^{t^{2} / 2} \\
&=e^{t^{2} / 2}
\end{aligned}$$

which is the mgf of a standard normal distribution. Therefore by uniqueness of moment generating functions, Proposition $1, Z \sim N(0,1)$.

---

**Reference**

- <https://digitalcommons.usu.edu/cgi/viewcontent.cgi?article=1014&context=gradreports>

